code/style-experiments/Hacl.Impl.Curve25519.Field51.fst
@@ -1,0 +1,395 @@
+module Hacl.Impl.Curve25519.Field51
+
+module ST = FStar.HyperStack.ST
+open FStar.HyperStack
+open FStar.HyperStack.All
+open Lib.Sequence
+open Lib.IntTypes
+open Lib.Buffer
+open FStar.Mul
+//open Lib.Utils
+
+let felem = lbuffer uint64 5ul
+let felem_wide = lbuffer uint128 5ul
+
+
+noextract 
+val as_nat: h:mem -> e:felem -> GTot nat 
+let as_nat h e = 
+    let s = as_seq h e in
+    let s0 =  uint_v (s.[0]) in
+    let s1 =  uint_v (s.[1]) in
+    let s2 =  uint_v (s.[2]) in
+    let s3 =  uint_v (s.[3]) in
+    let s4 =  uint_v (s.[4]) in
+    s0 + (s1 * pow2 51) + (s2 * pow2 102)  + (s3 * pow2 153)  + (s4 * pow2 204) 
+
+noextract 
+val wide_as_nat: h:mem -> e:felem_wide -> GTot nat 
+let wide_as_nat h e = 
+    let s = as_seq h e in
+    let s0 =  uint_v (s.[0]) in
+    let s1 =  uint_v (s.[1]) in
+    let s2 =  uint_v (s.[2]) in
+    let s3 =  uint_v (s.[3]) in
+    let s4 =  uint_v (s.[4]) in
+    s0 + (s1 * pow2 51) + (s2 * pow2 102)  + (s3 * pow2 153)  + (s4 * pow2 204) 
+
+
+inline_for_extraction
+val create_felem: unit -> StackInline felem
+		       (requires (fun _ -> True))
+		       (ensures (fun h0 f h1 -> stack_allocated f h0 h1 (Seq.create 5 (u64 0)) /\ 
+			 as_nat h1 f == 0))
+inline_for_extraction
+let create_felem () = create 5ul (u64 0)
+
+inline_for_extraction
+val create_wide: unit -> StackInline felem_wide
+		       (requires (fun _ -> True))
+		       (ensures (fun h0 f h1 -> stack_allocated f h0 h1 (Seq.create 5 (u128 0)) /\ wide_as_nat h1 f == 0))
+inline_for_extraction
+let create_wide () = create 5ul (u128 0)
+
+inline_for_extraction
+let mask51 = u64 0x7ffffffffffff
+
+
+
+inline_for_extraction
+val load_felem: f:felem -> u64s:lbuffer uint64 4ul -> Stack unit
+                   (requires (fun h -> live h u64s /\ live h f))
+		   (ensures (fun h0 _ h1 -> modifies (loc f) h0 h1))
+let load_felem f u64s = 
+    let f0l = u64s.(0ul) &. mask51 in
+    let f0h = u64s.(0ul) >>. 51ul in
+    let f1l = (u64s.(1ul) &. u64 0x3fffffffff) <<. 13ul in
+    let f1h = u64s.(1ul) >>. 38ul in
+    let f2l = (u64s.(2ul) &. u64 0x1fff) <<. 38ul in
+    let f2h = u64s.(2ul) >>. 13ul in
+    let f3l = (u64s.(3ul) &. u64 0x3fffffffff) <<. 13ul in
+    let f3h = u64s.(3ul) >>. 38ul in
+    f.(size 0) <- f0l;
+    f.(size 1) <- f0h ^. f1l;
+    f.(size 2) <- f1h ^. f2l;
+    f.(size 3) <- f2h ^. f3l;
+    f.(size 4) <- f3h
+
+inline_for_extraction
+val store_felem: u64s:lbuffer uint64 4ul -> f:felem -> Stack unit
+                   (requires (fun h -> live h f /\ live h u64s))
+		   (ensures (fun h0 _ h1 -> modifies (loc u64s) h0 h1))
+let store_felem u64s f = 
+    let f0 = f.(0ul) ^. (f.(1ul) <<. 51ul) in
+    let f1 = (f.(1ul) >>. 13ul) ^. (f.(2ul) <<. 38ul) in 
+    let f2 = (f.(2ul) >>. 13ul) ^. (f.(3ul) <<. 38ul) in 
+    let f3 = (f.(3ul) >>. 13ul) in
+    u64s.(0ul) <- f0;
+    u64s.(1ul) <- f1;
+    u64s.(2ul) <- f2;
+    u64s.(3ul) <- f3
+
+
+inline_for_extraction
+val set_bit1: f:felem -> i:size_t{v i < 255} -> Stack unit
+                   (requires (fun h -> live h f))
+		   (ensures (fun h0 _ h1 -> modifies (loc f) h0 h1))
+let set_bit1 f i = 
+    f.(i /. size 51) <- f.(i /. size 51) |. (u64 1 <<. (i %. size 51))
+
+inline_for_extraction
+val set_bit0: f:felem -> i:size_t{v i < 255} -> Stack unit
+                   (requires (fun h -> live h f))
+		   (ensures (fun h0 _ h1 -> modifies (loc f) h0 h1))
+let set_bit0 f i = 
+    f.(i /. size 51) <- f.(i /. size 51) &. lognot (u64 1 <<. (i %. size 51))
+
+inline_for_extraction
+val set_zero: f:felem -> Stack unit
+                   (requires (fun h -> live h f))
+		   (ensures (fun h0 _ h1 -> modifies (loc f) h0 h1))
+let set_zero f = memset f (u64 0) 5ul
+
+inline_for_extraction
+val copy_felem: f1:felem -> f2:felem -> Stack unit
+                   (requires (fun h -> live h f1 /\ live h f2))
+		   (ensures (fun h0 _ h1 -> modifies (loc f1) h0 h1))
+let copy_felem f1 f2 =
+    f1.(size 0) <- f2.(size 0);
+    f1.(size 1) <- f2.(size 1);
+    f1.(size 2) <- f2.(size 2);
+    f1.(size 3) <- f2.(size 3);
+    f1.(size 4) <- f2.(size 4)
+
+
+#reset-options "--z3rlimit 20"
+
+//inline_for_extraction
+[@ CInline]
+val fadd: out:felem ->  f1:felem  -> f2:felem  -> Stack unit
+                   (requires (fun h -> live h f1 /\ live h f2 /\ live h out /\
+		    (let s1 = as_seq h f1 in
+		     let s2 = as_seq h f2 in
+		     uint_v s1.[0] + uint_v s2.[0] <= maxint U64 /\ 
+		     uint_v s1.[1] + uint_v s2.[1] <= maxint U64 /\ 
+		     uint_v s1.[2] + uint_v s2.[2] <= maxint U64 /\
+		     uint_v s1.[3] + uint_v s2.[3] <= maxint U64 /\
+		     uint_v s1.[4] + uint_v s2.[4] <= maxint U64 )))
+		   (ensures (fun h0 _ h1 -> modifies (loc out) h0 h1 /\
+				         as_nat h1 out ==
+					 as_nat h0 f1 +
+					 as_nat h0 f2))		
+[@ CInline]
+let fadd out f1 f2 = 
+  let f10 = f1.(0ul) in
+  let f20 = f2.(0ul) in
+  let f11 = f1.(1ul) in
+  let f21 = f2.(1ul) in
+  let f12 = f1.(2ul) in
+  let f22 = f2.(2ul) in
+  let f13 = f1.(3ul) in
+  let f23 = f2.(3ul) in
+  let f14 = f1.(4ul) in
+  let f24 = f2.(4ul) in
+  out.(0ul) <- f10 +! f20;
+  out.(1ul) <- f11 +! f21;
+  out.(2ul) <- f12 +! f22;
+  out.(3ul) <- f13 +! f23;
+  out.(4ul) <- f14 +! f24
+
+//inline_for_extraction
+[@ CInline]
+val fsub: out:felem ->  f1:felem  -> f2:felem  -> Stack unit
+                   (requires (fun h -> live h f1 /\ live h f2 /\ live h out))
+		   (ensures (fun h0 _ h1 -> modifies (loc out) h0 h1 ))
+[@ CInline]
+let fsub out f1 f2 = 
+  let f10 = f1.(0ul) in
+  let f20 = f2.(0ul) in
+  let f11 = f1.(1ul) in
+  let f21 = f2.(1ul) in
+  let f12 = f1.(2ul) in
+  let f22 = f2.(2ul) in
+  let f13 = f1.(3ul) in
+  let f23 = f2.(3ul) in
+  let f14 = f1.(4ul) in
+  let f24 = f2.(4ul) in
+  out.(0ul) <- f10 +. (u64 0x3fffffffffff68) -. f20;
+  out.(1ul) <- f11 +. (u64 0x3ffffffffffff8) -. f21;
+  out.(2ul) <- f12 +. (u64 0x3ffffffffffff8) -. f22;
+  out.(3ul) <- f13 +. (u64 0x3ffffffffffff8) -. f23;
+  out.(4ul) <- f14 +. (u64 0x3ffffffffffff8) -. f24
+
+#reset-options "--z3rlimit 100"
+
+//[@ CInline]
+inline_for_extraction
+val smul_felem: out:felem_wide -> u1:uint64 -> f2:felem -> Stack unit
+                   (requires (fun h -> live h out /\ live h f2))
+		   (ensures (fun h0 _ h1 -> modifies (loc out) h0 h1 /\
+				         wide_as_nat h1 out ==
+				         uint_v u1 * as_nat h0 f2))
+[@ CInline]
+let smul_felem out u1 f2 = 
+  let f20 = f2.(size 0) in
+  let f21 = f2.(size 1) in
+  let f22 = f2.(size 2) in
+  let f23 = f2.(size 3) in
+  let f24 = f2.(size 4) in
+  out.(size 0) <- mul64_wide u1 f20;
+  out.(size 1) <- mul64_wide u1 f21;
+  out.(size 2) <- mul64_wide u1 f22;
+  out.(size 3) <- mul64_wide u1 f23;
+  out.(size 4) <- mul64_wide u1 f24
+
+//[@ CInline]
+inline_for_extraction
+val smul_add_felem: out:felem_wide -> u1:uint64 -> f2:felem -> Stack unit
+                   (requires (fun h -> live h out /\ live h f2 /\
+			       (let s1 = as_seq h out in
+				let s2 = as_seq h f2 in
+			        uint_v s1.[0] + uint_v u1 * uint_v s2.[0] <= maxint U128 /\ 
+			        uint_v s1.[1] + uint_v u1 * uint_v s2.[1] <= maxint U128 /\ 
+			        uint_v s1.[2] + uint_v u1 * uint_v s2.[2] <= maxint U128 /\ 
+			        uint_v s1.[3] + uint_v u1 * uint_v s2.[3] <= maxint U128 /\ 
+			        uint_v s1.[4] + uint_v u1 * uint_v s2.[4] <= maxint U128)))
+		   (ensures (fun h0 _ h1 -> modifies (loc out) h0 h1 /\
+				         wide_as_nat h1 out ==
+				         wide_as_nat h0 out +
+				         uint_v u1 * as_nat h0 f2))		
+
+[@ CInline]
+let smul_add_felem out u1 f2 = 
+  let f20 = f2.(size 0) in
+  let f21 = f2.(size 1) in
+  let f22 = f2.(size 2) in
+  let f23 = f2.(size 3) in
+  let f24 = f2.(size 4) in
+  let o0 = out.(size 0) in
+  let o1 = out.(size 1) in
+  let o2 = out.(size 2) in
+  let o3 = out.(size 3) in
+  let o4 = out.(size 4) in
+  out.(size 0) <- o0 +! mul64_wide u1 f20;
+  out.(size 1) <- o1 +! mul64_wide u1 f21;
+  out.(size 2) <- o2 +! mul64_wide u1 f22;
+  out.(size 3) <- o3 +! mul64_wide u1 f23;
+  out.(size 4) <- o4 +! mul64_wide u1 f24
+
+//inline_for_extraction
+[@ CInline]
+val mul_felem: out:felem_wide -> f1:felem -> r:felem -> r38:felem  -> Stack unit
+                   (requires (fun h -> live h out /\ live h f1 /\ live h r /\ live h r38))
+		   (ensures (fun h0 _ h1 -> modifies (loc out) h0 h1))
+[@ CInline]
+let mul_felem out f1 r r38 = 
+  push_frame();
+  let tmp = create 5ul (u64 0) in
+  smul_felem out f1.(size 0) r;
+  tmp.(size 0) <- r38.(size 4);
+  tmp.(size 1) <- r.(size 0);
+  tmp.(size 2) <- r.(size 1);
+  tmp.(size 3) <- r.(size 2);
+  tmp.(size 4) <- r.(size 3);
+  admit();
+  smul_add_felem out f1.(size 1) tmp;
+  tmp.(size 0) <- r38.(3ul);
+  tmp.(size 1) <- r38.(4ul);
+  tmp.(size 2) <- r.(0ul);
+  tmp.(size 3) <- r.(1ul);
+  tmp.(size 4) <- r.(2ul);
+  smul_add_felem out f1.(size 2) tmp;
+  tmp.(size 0) <- r38.(2ul);
+  tmp.(size 1) <- r38.(3ul);
+  tmp.(size 2) <- r38.(4ul);
+  tmp.(size 3) <- r.(0ul);
+  tmp.(size 4) <- r.(1ul);
+  smul_add_felem out f1.(size 3) tmp;
+  tmp.(size 0) <- r38.(1ul);
+  tmp.(size 1) <- r38.(2ul);
+  tmp.(size 2) <- r38.(3ul);
+  tmp.(size 3) <- r38.(4ul);
+  tmp.(size 4) <- r.(0ul);
+  smul_add_felem out f1.(size 4) tmp;
+  pop_frame()
+
+
+inline_for_extraction
+val carry51: l:uint64 -> cin:uint64 ->  (uint64 & uint64)
+let carry51 l cin = 
+    let l = l +. cin in
+    (l &. mask51, l >>. 51ul)
+
+inline_for_extraction
+val carry51_wide: l:uint128 -> cin:uint64 ->  (uint64 & uint64)
+let carry51_wide l cin = 
+    let l = l +. to_u128 cin in
+    (to_u64 l &. mask51, to_u64 (l >>. 51ul))
+
+
+//[@ CInline]
+inline_for_extraction
+val carry_wide: out:felem -> inp:felem_wide -> Stack unit
+                   (requires (fun h -> live h out /\ live h inp))
+		   (ensures (fun h0 _ h1 -> modifies (loc out) h0 h1))
+[@ CInline]
+let carry_wide out inp =
+  let i0 = inp.(size 0) in
+  let i1 = inp.(size 1) in
+  let i2 = inp.(size 2) in
+  let i3 = inp.(size 3) in
+  let i4 = inp.(size 4) in
+  let tmp0,carry = carry51_wide i0 (u64 0) in
+  let tmp1,carry = carry51_wide i1 carry in
+  let tmp2,carry = carry51_wide i2 carry in
+  let tmp3,carry = carry51_wide i3 carry in
+  let tmp4,carry = carry51_wide i4 carry in
+  let tmp0 = tmp0 +. (carry *. u64 19) in
+  out.(size 0) <- tmp0;
+  out.(size 1) <- tmp1;
+  out.(size 2) <- tmp2;
+  out.(size 3) <- tmp3;
+  out.(size 4) <- tmp4
+
+//[@ CInline]
+inline_for_extraction
+val carry_felem: f:felem -> Stack unit
+                   (requires (fun h -> live h f))
+		   (ensures (fun h0 _ h1 -> modifies (loc f) h0 h1))
+[@ CInline]
+let carry_felem f =
+  let f0 = f.(size 0) in
+  let f1 = f.(size 1) in
+  let f2 = f.(size 2) in
+  let f3 = f.(size 3) in
+  let f4 = f.(size 4) in
+  let tmp0,carry = carry51 f0 (u64 0) in
+  let tmp1,carry = carry51 f1 carry in
+  let tmp2,carry = carry51 f2 carry in
+  let tmp3,carry = carry51 f3 carry in
+  let tmp4 = f4 +. carry in
+  f.(size 0) <- tmp0;
+  f.(size 1) <- tmp1;
+  f.(size 2) <- tmp2;
+  f.(size 3) <- tmp3;
+  f.(size 4) <- tmp4
+
+//[@ CInline]
+inline_for_extraction
+val carry_top_felem: f:felem -> Stack unit
+                   (requires (fun h -> live h f))
+		   (ensures (fun h0 _ h1 -> modifies (loc f) h0 h1))
+[@ CInline]
+let carry_top_felem f =
+  let f0 = f.(size 0) in
+  let f1 = f.(size 1) in
+  let f2 = f.(size 2) in
+  let f3 = f.(size 3) in
+  let f4 = f.(size 4) in
+  let tmp4,carry = carry51 f4 (u64 0) in
+  let tmp0,carry = carry51 f0 (carry *. u64 19) in
+  let tmp1 = f1 +. carry in
+  f.(size 0) <- tmp0;
+  f.(size 1) <- tmp1;
+  f.(size 4) <- tmp4
+
+inline_for_extraction
+val fmul: out:felem -> f1:felem -> f2:felem -> Stack unit
+                   (requires (fun h -> live h out /\ live h f1 /\ live h f2))
+		   (ensures (fun h0 _ h1 -> modifies (loc out) h0 h1))
+[@ CInline]
+let fmul out f1 f2 =
+  push_frame();
+  let tmp = create_felem() in
+  let tmp_w = create_wide () in
+//  tmp.(0ul) <- f2.(0ul) *. u64 38;
+  tmp.(1ul) <- f2.(1ul) *. u64 38;
+  tmp.(2ul) <- f2.(2ul) *. u64 38;
+  tmp.(3ul) <- f2.(3ul) *. u64 38;
+  tmp.(4ul) <- f2.(4ul) *. u64 38;
+  mul_felem tmp_w f1 f2 tmp;
+  let carry = carry_wide out tmp_w in
+  carry_felem out;
+  carry_top_felem out;
+  carry_felem out;
+  pop_frame()
+
+inline_for_extraction
+val fmul1: out:felem -> f1:felem -> f2:uint64 -> Stack unit
+                   (requires (fun h -> live h out /\ live h f1))
+		   (ensures (fun h0 _ h1 -> modifies (loc out) h0 h1))
+[@ CInline]
+let fmul1 out f1 f2 =
+  push_frame();
+  let tmp_w = create_wide () in
+  smul_felem tmp_w f2 f1;
+  let carry = carry_wide out tmp_w in
+  pop_frame()
+
+inline_for_extraction
+val fsqr: out:felem -> f1:felem -> Stack unit
+                   (requires (fun h -> live h out /\ live h f1))
+		   (ensures (fun h0 _ h1 -> modifies (loc out) h0 h1))
+[@ CInline]
+let fsqr out f1 = fmul out f1 f1
+
