code/style-experiments/Hacl.Impl.Curve25519.Fields.fst
@@ -1,0 +1,145 @@
+module Hacl.Impl.Curve25519.Fields
+
+module ST = FStar.HyperStack.ST
+open FStar.HyperStack
+open FStar.HyperStack.All
+open Lib.IntTypes
+open Lib.Buffer
+module F51 = Hacl.Impl.Curve25519.Field51
+
+
+type field_spec = 
+  | M51
+
+
+unfold
+let limb (s:field_spec) =
+  match s with
+  | M51 -> uint64
+
+unfold
+let limb_zero (s:field_spec) : limb s=
+  match s with
+  | M51 -> u64 0
+
+unfold
+let wide (s:field_spec) =
+  match s with
+  | M51 -> uint128
+
+unfold
+let nlimb (s:field_spec) : size_t =
+  match s with
+  | M51 -> 5ul
+
+type felem (s:field_spec) = lbuffer (limb s) (nlimb s)
+type felem_wide (s:field_spec) = lbuffer (wide s) (nlimb s)
+
+
+noextract 
+val as_nat: #s:field_spec -> h:mem -> e:felem s-> GTot nat 
+let as_nat #s h (e:felem s) = 
+  match s with
+  | M51 -> F51.as_nat h e
+  
+inline_for_extraction
+val create_felem: s:field_spec -> StackInline (felem s)
+                   (requires (fun h -> True))
+		   (ensures (fun h0 f h1 -> stack_allocated f h0 h1 (Seq.create (v (nlimb s)) (limb_zero s)) /\ as_nat h1 f == 0))
+let create_felem s = 
+  match s with
+  | M51 -> (F51.create_felem ()) <: felem s
+
+
+
+inline_for_extraction
+val load_felem: #s:field_spec -> f:felem s -> u64s:lbuffer uint64 4ul -> Stack unit
+                   (requires (fun h -> live h f /\ live h u64s))
+		   (ensures (fun h0 _ h1 -> modifies (loc f) h0 h1))
+let load_felem (#s:field_spec) (f:felem s) (b:lbuffer uint64 4ul) =
+  match s with
+  | M51 -> F51.load_felem f b
+
+inline_for_extraction
+val store_felem: #s:field_spec -> b:lbuffer uint64 4ul -> f:felem s -> Stack unit
+                   (requires (fun h -> live h f /\ live h b))
+		   (ensures (fun h0 _ h1 -> modifies (loc b) h0 h1))
+let store_felem #s b f = 
+  match s with
+  | M51 -> F51.store_felem b f 
+
+inline_for_extraction
+val set_bit1: #s:field_spec -> f:felem s -> i:size_t{size_v i < 255} -> Stack unit
+                   (requires (fun h -> live h f))
+		   (ensures (fun h0 _ h1 -> modifies (loc f) h0 h1))
+let set_bit1 #s f i =
+  match s with
+  | M51 -> F51.set_bit1 f i
+
+inline_for_extraction
+val set_bit0: #s:field_spec -> f:felem s -> i:size_t{size_v i < 255} -> Stack unit
+                   (requires (fun h -> live h f))
+		   (ensures (fun h0 _ h1 -> modifies (loc f) h0 h1))
+let set_bit0 #s f i =
+  match s with
+  | M51 -> F51.set_bit0 f i
+
+
+inline_for_extraction
+val set_zero: #s:field_spec -> f:felem s -> Stack unit
+                   (requires (fun h -> live h f))
+		   (ensures (fun h0 _ h1 -> modifies (loc f) h0 h1))
+let set_zero (#s:field_spec) (f:felem s) = 
+  match s with
+  | M51 -> F51.set_zero f
+
+inline_for_extraction
+val copy_felem: #s:field_spec -> f:felem s -> f':felem s -> Stack unit
+                   (requires (fun h -> live h f /\ live h f'))
+		   (ensures (fun h0 _ h1 -> modifies (loc f) h0 h1))
+let copy_felem (#s:field_spec) (f:felem s) (f':felem s) = 
+  match s with
+  | M51 -> F51.copy_felem f f'
+
+inline_for_extraction
+val fadd: #s:field_spec -> out:felem s -> f1:felem s -> f2:felem s -> Stack unit
+                   (requires (fun h -> live h out /\ live h f1 /\ live h f2))
+		   (ensures (fun h0 _ h1 -> modifies (loc out) h0 h1))
+let fadd #s out f1 f2=
+  match s with
+  | M51 -> admit(); F51.fadd out f1 f2 
+
+inline_for_extraction
+val fsub: #s:field_spec -> out:felem s -> f1:felem s -> f2:felem s -> Stack unit
+                   (requires (fun h -> live h out /\ live h f1 /\ live h f2))
+		   (ensures (fun h0 _ h1 -> modifies (loc out) h0 h1))
+let fsub #s out f1 f2=
+  match s with
+  | M51 -> F51.fsub out f1 f2 
+
+
+inline_for_extraction
+val fmul: #s:field_spec -> out:felem s -> f1:felem s -> f2:felem s -> Stack unit
+                   (requires (fun h -> live h out /\ live h f1 /\ live h f2))
+		   (ensures (fun h0 _ h1 -> modifies (loc out) h0 h1 /\ live h1 out /\ live h1 f1 /\ live h1 f2))
+let fmul #s out f1 f2=
+  match s with
+  | M51 -> F51.fmul out f1 f2 
+
+inline_for_extraction
+val fmul1: #s:field_spec -> out:felem s -> f1:felem s -> f2:uint64 -> Stack unit
+                   (requires (fun h -> live h out /\ live h f1))
+		   (ensures (fun h0 _ h1 -> modifies (loc out) h0 h1 /\ live h1 out /\ live h1 f1))
+let fmul1 #s out f1 f2 =
+  match s with
+  | M51 -> F51.fmul1 out f1 f2 
+
+inline_for_extraction
+val fsqr: #s:field_spec -> out:felem s -> f1:felem s -> Stack unit
+                   (requires (fun h -> live h out /\ 
+				    live h f1))
+		   (ensures (fun h0 _ h1 -> modifies (loc out) h0 h1))
+let fsqr #s out f1 =
+  match s with
+  | M51 -> F51.fsqr out f1 
+
